Reorder args for currying, start Hoare triple implementation

Blocks.thy
@@ -11,82 +11,81 @@ fun phi_lookup :: "llvm_label option \<Rightarrow> (llvm_label * llvm_value_ref)
     some_or_err (map_of ls prev) phi_label_not_found
   }"
 
-definition execute_phi :: "state \<Rightarrow> llvm_label option \<Rightarrow> llvm_register_name \<Rightarrow> (llvm_label * llvm_value_ref) list \<Rightarrow> state result" where
-  "execute_phi s prev name values = do {
+definition execute_phi :: "llvm_label option \<Rightarrow> llvm_register_name \<Rightarrow> (llvm_label * llvm_value_ref) list \<Rightarrow> state \<Rightarrow> state result" where
+  "execute_phi prev name values s = do {
     v \<leftarrow> phi_lookup prev values;
     v' \<leftarrow> get_register s v;
-    return (set_register s name v')
+    return (set_register name v' s)
   }"
 
-lemma wp_execute_phi_intro[THEN consequence, wp_intro]:
+lemma phi_wp_intro[THEN consequence, wp_intro]:
   assumes "distinct (map fst values)"
-  assumes "p = Some prev"
-  assumes "map_of values prev = Some v"
-  assumes "register_\<alpha> s v = Some v'"
-  shows "wp (execute_phi s p name values) (\<lambda>s'. register_\<alpha> s' = (register_\<alpha> s)(reg name := Some v') \<and> memory_\<alpha> s' = memory_\<alpha> s)"
+  assumes "\<exists>p' v v'. p = Some p' \<and> map_of values p' = Some v \<and> register_\<alpha> s v = Some v'"
+  shows "wp (execute_phi p name values s) (\<lambda>s'. \<exists>p' v v'. p = Some p' \<and> map_of values p' = Some v \<and> register_\<alpha> s v = Some v' \<and> register_\<alpha> s' = (register_\<alpha> s)(reg name := Some v') \<and> memory_\<alpha> s' = memory_\<alpha> s)"
   unfolding execute_phi_def
   apply simp
   using assms
-  by (intro wp_intro; auto)
+  apply (intro wp_intro; auto)
+  by (metis eq_key_imp_eq_value)
 
 
 
 section "Single block"
 
-fun execute_block :: "state \<Rightarrow> llvm_label option \<Rightarrow> llvm_instruction_block \<Rightarrow> (state * llvm_block_return) result" where
-  "execute_block s previous ((phi name type values)#ps, is, t) = do {
-    s' \<leftarrow> execute_phi s previous name values;
-    execute_block s' previous (ps, is, t)
+fun execute_block :: "llvm_label option \<Rightarrow> llvm_instruction_block \<Rightarrow> state \<Rightarrow> (state * llvm_block_return) result" where
+  "execute_block previous ((phi name type values)#ps, is, t) s = do {
+    s' \<leftarrow> execute_phi previous name values s;
+    execute_block previous (ps, is, t) s'
   }"
-| "execute_block s previous ([], i#is, t) = do {
-    s' \<leftarrow> execute_instruction s i;
-    execute_block s' previous ([], is, t)
+| "execute_block previous ([], i#is, t) s = do {
+    s' \<leftarrow> execute_instruction i s;
+    execute_block previous ([], is, t) s'
   }"
-| "execute_block s previous (_, _, br_i1 v l1 l2) = do {
+| "execute_block previous (_, _, br_i1 v l1 l2) s = do {
     val \<leftarrow> get_register s v;
     label \<leftarrow> (case val of (vi1 b) \<Rightarrow> ok (if b then l1 else l2) | _ \<Rightarrow> err incompatible_types);
     return (s, branch_label label)
   }"
-| "execute_block s previous (_, _, br_label l) = return (s, branch_label l)"
-| "execute_block s previous (_, _, ret t v) = do {
+| "execute_block previous (_, _, br_label l) s = return (s, branch_label l)"
+| "execute_block previous (_, _, ret t v) s = do {
     res \<leftarrow> get_register s v;
     return (s, return_value res)
   }"
 
-lemma wp_execute_phi_block_intro[wp_intro]:
-  assumes "wp (execute_phi s p name values) (\<lambda>s'. wp (execute_block s' p (ps, is, t)) Q)"
-  shows "wp (execute_block s p ((phi name type values)#ps, is, t)) Q"
+lemma block_phi_wp_intro[wp_intro]:
+  assumes "wp (execute_phi p name values s) (\<lambda>s'. wp (execute_block p (ps, is, t) s') Q)"
+  shows "wp (execute_block p ((phi name type values)#ps, is, t) s) Q"
   using assms
   by (simp; rule wp_intro; simp)
 
-lemma wp_execute_intruction_block_intro[wp_intro]:
-  assumes "wp (execute_instruction s i) (\<lambda>s'. wp (execute_block s' p ([], is, t)) Q)"
-  shows "wp (execute_block s p ([], i#is, t)) Q"
+lemma block_instr_wp_intro[wp_intro]:
+  assumes "wp (execute_instruction i s) (\<lambda>s'. wp (execute_block p ([], is, t) s') Q)"
+  shows "wp (execute_block p ([], i#is, t) s) Q"
   using assms
   by (simp; rule wp_intro; simp)
 
-lemma wp_execute_return_block_intro[THEN consequence, wp_intro]:
+lemma block_ret_wp_intro[THEN consequence, wp_intro]:
   assumes "\<exists>v. register_\<alpha> s value = Some v"
-  shows "wp (execute_block s p ([], [], ret type value)) (\<lambda>(s', r). s' = s \<and> (\<exists>v. register_\<alpha> s value = Some v \<and> r = return_value v))"
+  shows "wp (execute_block p ([], [], ret type value) s) (\<lambda>(s', r). s' = s \<and> (\<exists>v. register_\<alpha> s value = Some v \<and> r = return_value v))"
   using assms
   by (simp; intro wp_intro wp_return_intro; simp)
 
-lemma wp_execute_branch_label_block_intro[THEN consequence, wp_intro]:
-  shows "wp (execute_block s p ([], [], br_label l)) (\<lambda>(s', r). s' = s \<and> r = branch_label l)"
+lemma block_br_label_wp_intro[THEN consequence, wp_intro]:
+  shows "wp (execute_block p ([], [], br_label l) s) (\<lambda>(s', r). s' = s \<and> r = branch_label l)"
   by (simp; rule wp_return_intro; simp)
 
-lemma wp_execute_branch_i1_block_intro[THEN consequence, wp_intro]:
+lemma block_br_i1_wp_intro[THEN consequence, wp_intro]:
   assumes "\<exists>b. register_\<alpha> s value = Some (vi1 b)"
-  shows "wp (execute_block s p ([], [], br_i1 value l1 l2)) (\<lambda>(s', r). s' = s \<and> (\<exists>b. register_\<alpha> s value = Some (vi1 b) \<and> r = branch_label (if b then l1 else l2)))"
+  shows "wp (execute_block p ([], [], br_i1 value l1 l2) s) (\<lambda>(s', r). s' = s \<and> (\<exists>b. register_\<alpha> s value = Some (vi1 b) \<and> r = branch_label (if b then l1 else l2)))"
   using assms
   by (simp; intro wp_intro; auto; intro wp_intro wp_return_intro; auto)
 
 
 section "Multiple blocks"
 
-partial_function (tailrec) execute_blocks :: "state \<Rightarrow> llvm_label option \<Rightarrow> llvm_label option \<Rightarrow> llvm_instruction_block \<Rightarrow> llvm_labeled_blocks \<Rightarrow> (state * llvm_value option) result" where
-  "execute_blocks state previous current block labeled_blocks =
-    (case execute_block state previous block of
+partial_function (tailrec) execute_blocks :: "llvm_label option \<Rightarrow> llvm_label option \<Rightarrow> llvm_instruction_block \<Rightarrow> llvm_labeled_blocks \<Rightarrow> state \<Rightarrow> (state * llvm_value option) result" where
+  "execute_blocks previous current block labeled_blocks state =
+    (case execute_block previous block state of
       err e \<Rightarrow> err e
     | ok (s', br) \<Rightarrow>
       (case br of
@@ -94,16 +93,16 @@ partial_function (tailrec) execute_blocks :: "state \<Rightarrow> llvm_label opt
       | branch_label l \<Rightarrow>
         (case map_of labeled_blocks l of
           None \<Rightarrow> err unknown_label
-        | Some b' \<Rightarrow> execute_blocks s' current (Some l) b' labeled_blocks
+        | Some b' \<Rightarrow> execute_blocks current (Some l) b' labeled_blocks s'
         )
       )
     )"
 
 lemmas [code] = execute_blocks.simps
 
-fun execute_function :: "state \<Rightarrow> llvm_function \<Rightarrow> (llvm_value option) result" where
-  "execute_function s (func _ is ls) = do {
-    (_, r) \<leftarrow> execute_blocks s None None is ls;
+fun execute_function :: "llvm_function \<Rightarrow> state \<Rightarrow> (llvm_value option) result" where
+  "execute_function (func _ is ls) s = do {
+    (_, r) \<leftarrow> execute_blocks None None is ls s;
     return r
   }"
 
