Instructions.thy
@@ -16,14 +16,14 @@ lemma wp_case_value_addr_intro[wp_intro]:
 
 section "Memory instructions"
 
-definition execute_alloca :: "state \<Rightarrow> llvm_register_name \<Rightarrow> state result" where
-  "execute_alloca s name = do {
+definition execute_alloca :: "llvm_register_name \<Rightarrow> state \<Rightarrow> state result" where
+  "execute_alloca name s = do {
       (s', a) \<leftarrow> return (allocate_stack s);
-      return (set_register s' name (addr a))
+      return (set_register name (addr a) s')
     }"
 
-lemma wp_execute_alloca_intro[THEN consequence, wp_intro]:
-  "wp (execute_alloca s name) (\<lambda>s'. \<exists>a. (register_\<alpha> s' = (register_\<alpha> s)(reg name := Some (addr a)) \<and> memory_\<alpha> s' = (memory_\<alpha> s)(a := Some None) \<and> memory_\<alpha> s a = None))"
+lemma alloca_wp_intro[THEN consequence, wp_intro]:
+  "wp (execute_alloca name s) (\<lambda>s'. \<exists>a. (register_\<alpha> s' = (register_\<alpha> s)(reg name := Some (addr a)) \<and> memory_\<alpha> s' = (memory_\<alpha> s)(a := Some None) \<and> memory_\<alpha> s a = None))"
   unfolding execute_alloca_def
   by (intro wp_intro; auto)
 
@@ -34,39 +34,37 @@ fun get_address_from_pointer :: "state \<Rightarrow> llvm_pointer \<Rightarrow> 
     (case a of (addr a') \<Rightarrow> ok a' | _ \<Rightarrow> err not_an_address)
   }"
 
-definition execute_store :: "state \<Rightarrow> llvm_value_ref \<Rightarrow> llvm_pointer \<Rightarrow> state result" where
-  "execute_store s v p = do {
+definition execute_store :: "llvm_value_ref \<Rightarrow> llvm_pointer \<Rightarrow> state \<Rightarrow> state result" where
+  "execute_store v p s = do {
     address \<leftarrow> get_address_from_pointer s p;
     value \<leftarrow> get_register s v;
-    set_memory s address value
+    set_memory address value s
   }"
 
-lemma wp_execute_store_intro[THEN consequence, wp_intro]:
+lemma store_wp_intro[THEN consequence, wp_intro]:
   assumes "\<exists>a. register_\<alpha> s pointer = Some (addr a) \<and> memory_\<alpha> s a \<noteq> None"
   assumes "register_\<alpha> s value \<noteq> None"
-  shows "wp (execute_store s value pointer) (\<lambda>s'. \<exists>a v. register_\<alpha> s pointer = Some (addr a) \<and> register_\<alpha> s value = Some v \<and> memory_\<alpha> s' = (memory_\<alpha> s)(a := Some (Some v)) \<and> register_\<alpha> s = register_\<alpha> s')"
+  shows "wp (execute_store value pointer s) (\<lambda>s'. \<exists>a v. register_\<alpha> s pointer = Some (addr a) \<and> register_\<alpha> s value = Some v \<and> memory_\<alpha> s' = (memory_\<alpha> s)(a := Some (Some v)) \<and> register_\<alpha> s = register_\<alpha> s')"
   unfolding execute_store_def
   using assms
   apply simp
   by (intro wp_intro; auto)
 
 
-definition execute_load :: "state \<Rightarrow> llvm_register_name \<Rightarrow> llvm_pointer \<Rightarrow> state result" where
-  "execute_load s n p = do {
+definition execute_load :: "llvm_register_name \<Rightarrow> llvm_pointer \<Rightarrow> state \<Rightarrow> state result" where
+  "execute_load n p s = do {
     a \<leftarrow> get_address_from_pointer s p;
     v \<leftarrow> get_memory s a;
-    return (set_register s n v)
+    return (set_register n v s)
   }"
 
-lemma wp_execute_load_intro[THEN consequence, wp_intro]:
+lemma load_wp_intro[THEN consequence, wp_intro]:
   assumes "\<exists>a v. register_\<alpha> s pointer = Some (addr a) \<and> memory_\<alpha> s a = Some (Some v)"
-  shows "wp (execute_load s name pointer) (\<lambda>s'. \<exists>a v. register_\<alpha> s pointer = Some (addr a) \<and> memory_\<alpha> s a = Some (Some v) \<and> memory_\<alpha> s' = memory_\<alpha> s \<and> register_\<alpha> s' = (register_\<alpha> s)(reg name := Some v))"
+  shows "wp (execute_load name pointer s) (\<lambda>s'. \<exists>a v. register_\<alpha> s pointer = Some (addr a) \<and> memory_\<alpha> s a = Some (Some v) \<and> memory_\<alpha> s' = memory_\<alpha> s \<and> register_\<alpha> s' = (register_\<alpha> s)(reg name := Some v))"
   unfolding execute_load_def
   using assms
   apply simp
   by (intro wp_intro; auto)
-
-thm wp_execute_load_intro[THEN consequence]
 
 
 section "Add instruction"
@@ -122,25 +120,25 @@ fun add_values :: "llvm_add_wrap \<Rightarrow> llvm_value \<Rightarrow> llvm_val
 | "add_values _ _ _ = err incompatible_types"
 
 
-definition execute_add :: "state \<Rightarrow> llvm_register_name \<Rightarrow> llvm_add_wrap \<Rightarrow> llvm_value_ref \<Rightarrow> llvm_value_ref \<Rightarrow> state result" where
-  "execute_add s name wrap v1 v2 = do {
+definition execute_add :: "llvm_register_name \<Rightarrow> llvm_add_wrap \<Rightarrow> llvm_value_ref \<Rightarrow> llvm_value_ref \<Rightarrow> state \<Rightarrow> state result" where
+  "execute_add name wrap v1 v2 s = do {
     v1' \<leftarrow> get_register s v1;
     v2' \<leftarrow> get_register s v2;
     res \<leftarrow> add_values wrap v1' v2';
-    return (set_register s name res)
+    return (set_register name res s)
   }"
 
 
-lemma wp_execute_add_32_intro[THEN consequence, wp_intro]:
+lemma add32_wp_intro[THEN consequence, wp_intro]:
   assumes "\<exists>v1' v2'. register_\<alpha> s v1 = Some (vi32 v1') \<and> register_\<alpha> s v2 = Some (vi32 v2') \<and> add_no_poison32 wrap v1' v2'"
-  shows "wp (execute_add s name wrap v1 v2) (\<lambda>s'. \<exists>v1' v2'. register_\<alpha> s v1 = Some (vi32 v1') \<and> register_\<alpha> s v2 = Some (vi32 v2') \<and> memory_\<alpha> s' = memory_\<alpha> s \<and> register_\<alpha> s' = (register_\<alpha> s)(reg name := Some (vi32 (v1' + v2'))))"
+  shows "wp (execute_add name wrap v1 v2 s) (\<lambda>s'. \<exists>v1' v2'. register_\<alpha> s v1 = Some (vi32 v1') \<and> register_\<alpha> s v2 = Some (vi32 v2') \<and> memory_\<alpha> s' = memory_\<alpha> s \<and> register_\<alpha> s' = (register_\<alpha> s)(reg name := Some (vi32 (v1' + v2'))))"
   using assms
   unfolding execute_add_def
   by (intro wp_intro; simp; auto; intro wp_intro; simp)
 
-lemma wp_execute_add_64_intro[THEN consequence, wp_intro]:
+lemma add64_wp_intro[THEN consequence, wp_intro]:
   assumes "\<exists>v1' v2'. register_\<alpha> s v1 = Some (vi64 v1') \<and> register_\<alpha> s v2 = Some (vi64 v2') \<and> add_no_poison64 wrap v1' v2'"
-  shows "wp (execute_add s name wrap v1 v2) (\<lambda>s'. \<exists>v1' v2'. register_\<alpha> s v1 = Some (vi64 v1') \<and> register_\<alpha> s v2 = Some (vi64 v2') \<and> memory_\<alpha> s' = memory_\<alpha> s \<and> register_\<alpha> s' = (register_\<alpha> s)(reg name := Some (vi64 (v1' + v2'))))"
+  shows "wp (execute_add name wrap v1 v2 s) (\<lambda>s'. \<exists>v1' v2'. register_\<alpha> s v1 = Some (vi64 v1') \<and> register_\<alpha> s v2 = Some (vi64 v2') \<and> memory_\<alpha> s' = memory_\<alpha> s \<and> register_\<alpha> s' = (register_\<alpha> s)(reg name := Some (vi64 (v1' + v2'))))"
   using assms
   unfolding execute_add_def
   by (intro wp_intro; simp; auto; intro wp_intro; simp)
@@ -188,24 +186,24 @@ fun compare_values_sign :: "llvm_same_sign \<Rightarrow> llvm_compare_condition 
 | "compare_values_sign True c (vi64 a) (vi64 b) = (if same_signs (sint a) (sint b) then compare_values c (vi64 a) (vi64 b) else ok poison)"
 | "compare_values_sign True c _ _ = err incompatible_types"
 
-definition execute_icmp :: "state \<Rightarrow> llvm_register_name \<Rightarrow> llvm_same_sign \<Rightarrow> llvm_compare_condition \<Rightarrow> llvm_value_ref \<Rightarrow> llvm_value_ref \<Rightarrow> state result" where
-  "execute_icmp s name same_sign cond v1 v2 = do {
+definition execute_icmp :: "llvm_register_name \<Rightarrow> llvm_same_sign \<Rightarrow> llvm_compare_condition \<Rightarrow> llvm_value_ref \<Rightarrow> llvm_value_ref \<Rightarrow> state \<Rightarrow> state result" where
+  "execute_icmp name same_sign cond v1 v2 s = do {
     v1' \<leftarrow> get_register s v1;
     v2' \<leftarrow> get_register s v2;
     res \<leftarrow> compare_values_sign same_sign cond v1' v2';
-    return (set_register s name res)
+    return (set_register name res s)
   }"
 
-lemma wp_execute_icmp_32_intro[THEN consequence, wp_intro]:
+lemma icmp32_wp_intro[THEN consequence, wp_intro]:
   assumes "\<exists>v1' v2'. register_\<alpha> s v1 = Some (vi32 v1') \<and> register_\<alpha> s v2 = Some (vi32 v2') \<and> (if ss then same_signs (sint v1') (sint v2') else True)"
-  shows "wp (execute_icmp s name ss cond v1 v2) (\<lambda>s'. \<exists>v1' v2'. register_\<alpha> s v1 = Some (vi32 v1') \<and> register_\<alpha> s v2 = Some (vi32 v2') \<and> memory_\<alpha> s' = memory_\<alpha> s \<and> register_\<alpha> s' = (register_\<alpha> s)(reg name := Some (compare_values_32 cond v1' v2')))"
+  shows "wp (execute_icmp name ss cond v1 v2 s) (\<lambda>s'. \<exists>v1' v2'. register_\<alpha> s v1 = Some (vi32 v1') \<and> register_\<alpha> s v2 = Some (vi32 v2') \<and> memory_\<alpha> s' = memory_\<alpha> s \<and> register_\<alpha> s' = (register_\<alpha> s)(reg name := Some (compare_values_32 cond v1' v2')))"
   using assms
   unfolding execute_icmp_def
   by (cases ss; intro wp_intro; auto; intro wp_intro; auto)
 
-lemma wp_execute_icmp_64_intro[THEN consequence, wp_intro]:
+lemma icmp64_wp_intro[THEN consequence, wp_intro]:
   assumes "\<exists>v1' v2'. register_\<alpha> s v1 = Some (vi64 v1') \<and> register_\<alpha> s v2 = Some (vi64 v2') \<and> (if ss then same_signs (sint v1') (sint v2') else True)"
-  shows "wp (execute_icmp s name ss cond v1 v2) (\<lambda>s'. \<exists>v1' v2'. register_\<alpha> s v1 = Some (vi64 v1') \<and> register_\<alpha> s v2 = Some (vi64 v2') \<and> memory_\<alpha> s' = memory_\<alpha> s \<and> register_\<alpha> s' = (register_\<alpha> s)(reg name := Some (compare_values_64 cond v1' v2')))"
+  shows "wp (execute_icmp name ss cond v1 v2 s) (\<lambda>s'. \<exists>v1' v2'. register_\<alpha> s v1 = Some (vi64 v1') \<and> register_\<alpha> s v2 = Some (vi64 v2') \<and> memory_\<alpha> s' = memory_\<alpha> s \<and> register_\<alpha> s' = (register_\<alpha> s)(reg name := Some (compare_values_64 cond v1' v2')))"
   using assms
   unfolding execute_icmp_def
   by (cases ss; intro wp_intro; auto; intro wp_intro; auto)
@@ -214,27 +212,27 @@ lemma wp_execute_icmp_64_intro[THEN consequence, wp_intro]:
 
 section "Instruction wrapper"
 
-fun execute_instruction :: "state \<Rightarrow> llvm_instruction \<Rightarrow> state result" where
-  (* Allocate new memory value on the stack, and set the specified SSA name to its address. *)
-  "execute_instruction s (alloca name type align) = execute_alloca s name"
+fun execute_instruction :: "llvm_instruction \<Rightarrow> state \<Rightarrow> state result" where
+  (* Allocate new memory value on the stack, and set the specified register to its address. *)
+  "execute_instruction (alloca name type align) s = execute_alloca name s"
   (* Read address from pointer and store value in the stack or the heap. *)
-| "execute_instruction s (store type value pointer align) = execute_store s value pointer"
+| "execute_instruction (store type value pointer align) s = execute_store value pointer s"
   (* Read address from pointer and load value from either the stack or the heap. *)
-| "execute_instruction s (load name type pointer align) = execute_load s name pointer"
-  (* Get values, add according to wrap option (or poison), and store at SSA name. *)
-| "execute_instruction s (add name wrap type v1 v2) = execute_add s name wrap v1 v2"
-  (* Get values, do comparison, and store at SSA name. *)
-| "execute_instruction s (icmp name same_sign cond type v1 v2) = execute_icmp s name same_sign cond v1 v2"
+| "execute_instruction (load name type pointer align) s = execute_load name pointer s"
+  (* Get values, add according to wrap option (or poison), and store in register. *)
+| "execute_instruction (add name wrap type v1 v2) s = execute_add name wrap v1 v2 s"
+  (* Get values, do comparison, and store in register. *)
+| "execute_instruction (icmp name same_sign cond type v1 v2) s = execute_icmp name same_sign cond v1 v2 s"
 
-lemma [wp_intro]: "wp (execute_alloca s name) Q \<Longrightarrow> wp (execute_instruction s (alloca name type align)) Q"
+lemma [wp_intro]: "wp (execute_alloca name s) Q \<Longrightarrow> wp (execute_instruction (alloca name type align) s) Q"
   by simp
-lemma [wp_intro]: "wp (execute_store s value pointer) Q \<Longrightarrow> wp (execute_instruction s (store type value pointer align)) Q"
+lemma [wp_intro]: "wp (execute_store value pointer s) Q \<Longrightarrow> wp (execute_instruction (store type value pointer align) s) Q"
   by simp
-lemma [wp_intro]: "wp (execute_load s name pointer) Q \<Longrightarrow> wp (execute_instruction s (load name type pointer align)) Q"
+lemma [wp_intro]: "wp (execute_load name pointer s) Q \<Longrightarrow> wp (execute_instruction (load name type pointer align) s) Q"
   by simp
-lemma [wp_intro]: "wp (execute_add s name wrap v1 v2) Q \<Longrightarrow> wp (execute_instruction s (add name wrap type v1 v2)) Q"
+lemma [wp_intro]: "wp (execute_add name wrap v1 v2 s) Q \<Longrightarrow> wp (execute_instruction (add name wrap type v1 v2) s) Q"
   by simp
-lemma [wp_intro]: "wp (execute_icmp s name same_sign cond v1 v2) Q \<Longrightarrow> wp (execute_instruction s (icmp name same_sign cond type v1 v2)) Q"
+lemma [wp_intro]: "wp (execute_icmp name same_sign cond v1 v2 s) Q \<Longrightarrow> wp (execute_instruction (icmp name same_sign cond type v1 v2) s) Q"
   by simp
 
 end
