Hoare.thy
@@ -1,0 +1,201 @@
+theory Hoare
+  imports "Blocks"
+begin
+
+section "Definitions"
+
+definition hoare :: "('a \<Rightarrow> bool) \<Rightarrow> ('a \<Rightarrow> 'b result) \<Rightarrow> ('b \<Rightarrow> bool) \<Rightarrow> bool" where
+  "hoare P c Q \<equiv> (\<forall>x. P x \<longrightarrow> wp (c x) Q)"
+
+definition state_marker :: "('a \<Rightarrow> bool) \<Rightarrow> ('a \<Rightarrow> bool)" where
+  "state_marker P \<equiv> P"
+
+
+lemma hoare_intro:
+  assumes "\<And>s. state_marker P s \<Longrightarrow> wp (c s) Q"
+  shows "hoare P c Q"
+  using assms
+  unfolding hoare_def state_marker_def
+  by simp
+
+lemma hoare_elim:
+  assumes "hoare P c Q" and "P s"
+  shows "wp (c s) Q"
+  using assms
+  unfolding hoare_def
+  by simp
+
+
+lemma vcg:
+  assumes "state_marker P s" and "hoare P c Q"
+  shows "wp (c s) Q"
+  using assms
+  unfolding hoare_def state_marker_def
+  by simp
+
+
+lemma hoare_consequence:
+  assumes assm: "hoare P c Q"
+  assumes pre:  "\<And>s. P' s \<Longrightarrow> P s"
+  assumes post: "\<And>s. Q s \<Longrightarrow> Q' s"
+  shows "hoare P' c Q'"
+  using assms consequence
+  unfolding hoare_def
+  by blast
+
+
+
+section "Instructions specifications"
+
+named_theorems hoare_specs
+
+lemma alloca_spec[hoare_specs]:
+  "hoare
+    (\<lambda>s'. s' = s)
+    (execute_alloca n)
+    (\<lambda>s'. \<exists>a. (register_\<alpha> s') = (register_\<alpha> s)(reg n := Some (addr a)) \<and> (memory_\<alpha> s') = (memory_\<alpha> s)(a := Some None) \<and> memory_\<alpha> s a = None)"
+  apply (rule hoare_intro)
+  apply (rule alloca_wp_intro)
+  by (auto simp: state_marker_def)
+
+lemma store_spec[hoare_specs]:
+  "hoare
+    (\<lambda>s'. \<exists>a. s' = s \<and> register_\<alpha> s pointer = Some (addr a) \<and> memory_\<alpha> s a \<noteq> None \<and> register_\<alpha> s value \<noteq> None)
+    (execute_store value pointer)
+    (\<lambda>s'. \<exists>a v. register_\<alpha> s pointer = Some (addr a) \<and> register_\<alpha> s value = Some v \<and> memory_\<alpha> s' = (memory_\<alpha> s)(a := Some (Some v)) \<and> register_\<alpha> s = register_\<alpha> s')"
+  apply (rule hoare_intro)
+  apply (rule store_wp_intro)
+  by (auto simp: state_marker_def)
+
+lemma load_spec[hoare_specs]:
+  "hoare
+    (\<lambda>s'. \<exists>a v. s' = s \<and> register_\<alpha> s pointer = Some (addr a) \<and> memory_\<alpha> s a = Some (Some v))
+    (execute_load name pointer)
+    (\<lambda>s'. \<exists>a v. register_\<alpha> s pointer = Some (addr a) \<and> memory_\<alpha> s a = Some (Some v) \<and> memory_\<alpha> s' = memory_\<alpha> s \<and> register_\<alpha> s' = (register_\<alpha> s)(reg name := Some v))"
+  apply (rule hoare_intro)
+  apply (rule load_wp_intro)
+  by (auto simp: state_marker_def)
+
+lemma add32_spec[hoare_specs]:
+  "hoare
+    (\<lambda>s'. \<exists>v1' v2'. s' = s \<and> register_\<alpha> s v1 = Some (vi32 v1') \<and> register_\<alpha> s v2 = Some (vi32 v2') \<and> add_no_poison32 wrap v1' v2')
+    (execute_add name wrap v1 v2)
+    (\<lambda>s'. \<exists>v1' v2'. register_\<alpha> s v1 = Some (vi32 v1') \<and> register_\<alpha> s v2 = Some (vi32 v2') \<and> memory_\<alpha> s' = memory_\<alpha> s \<and> register_\<alpha> s' = (register_\<alpha> s)(reg name := Some (vi32 (v1' + v2'))))"
+  apply (rule hoare_intro)
+  apply (rule add32_wp_intro)
+  by (auto simp: state_marker_def)
+
+lemma add64_spec[hoare_specs]:
+  "hoare
+    (\<lambda>s'. \<exists>v1' v2'. s' = s \<and> register_\<alpha> s v1 = Some (vi64 v1') \<and> register_\<alpha> s v2 = Some (vi64 v2') \<and> add_no_poison64 wrap v1' v2')
+    (execute_add name wrap v1 v2)
+    (\<lambda>s'. \<exists>v1' v2'. register_\<alpha> s v1 = Some (vi64 v1') \<and> register_\<alpha> s v2 = Some (vi64 v2') \<and> memory_\<alpha> s' = memory_\<alpha> s \<and> register_\<alpha> s' = (register_\<alpha> s)(reg name := Some (vi64 (v1' + v2'))))"
+  apply (rule hoare_intro)
+  apply (rule add64_wp_intro)
+  by (auto simp: state_marker_def)
+
+lemma icmp32_spec[hoare_specs]:
+  "hoare
+    (\<lambda>s'. \<exists>v1' v2'. s' = s \<and> register_\<alpha> s v1 = Some (vi32 v1') \<and> register_\<alpha> s v2 = Some (vi32 v2') \<and> (if ss then same_signs (sint v1') (sint v2') else True))
+    (execute_icmp name ss cond v1 v2)
+    (\<lambda>s'. \<exists>v1' v2'. register_\<alpha> s v1 = Some (vi32 v1') \<and> register_\<alpha> s v2 = Some (vi32 v2') \<and> memory_\<alpha> s' = memory_\<alpha> s \<and> register_\<alpha> s' = (register_\<alpha> s)(reg name := Some (compare_values_32 cond v1' v2')))"
+  apply (rule hoare_intro)
+  apply (rule wp_intro)
+  by (auto simp: state_marker_def)
+
+lemma icmp64_spec[hoare_specs]:
+  "hoare
+    (\<lambda>s'. \<exists>v1' v2'. s' = s \<and> register_\<alpha> s v1 = Some (vi64 v1') \<and> register_\<alpha> s v2 = Some (vi64 v2') \<and> (if ss then same_signs (sint v1') (sint v2') else True))
+    (execute_icmp name ss cond v1 v2)
+    (\<lambda>s'. \<exists>v1' v2'. register_\<alpha> s v1 = Some (vi64 v1') \<and> register_\<alpha> s v2 = Some (vi64 v2') \<and> memory_\<alpha> s' = memory_\<alpha> s \<and> register_\<alpha> s' = (register_\<alpha> s)(reg name := Some (compare_values_64 cond v1' v2')))"
+  apply (rule hoare_intro)
+  apply (rule icmp64_wp_intro)
+  by (auto simp: state_marker_def)
+
+
+lemma phi_spec[hoare_specs]:
+  "hoare
+    (\<lambda>s'. \<exists>p' v v'. s' = s \<and> distinct (map fst values) \<and> p = Some p' \<and> map_of values p' = Some v \<and> register_\<alpha> s v = Some v')
+    (execute_phi p name values)
+    (\<lambda>s'. \<exists>p' v v'. p = Some p' \<and> map_of values p' = Some v \<and> register_\<alpha> s v = Some v' \<and> register_\<alpha> s' = (register_\<alpha> s)(reg name := Some v') \<and> memory_\<alpha> s' = memory_\<alpha> s)"
+  apply (rule hoare_intro)
+  apply (rule phi_wp_intro)
+  apply (auto simp: state_marker_def)
+  by blast
+
+lemma [hoare_specs]: "hoare P (execute_alloca name) Q \<Longrightarrow> hoare P (execute_instruction (alloca name type align)) Q"
+  unfolding hoare_def by simp
+lemma [hoare_specs]: "hoare P (execute_store value pointer) Q \<Longrightarrow> hoare P (execute_instruction (store type value pointer align)) Q"
+  unfolding hoare_def by simp
+lemma [hoare_specs]: "hoare P (execute_load name pointer) Q \<Longrightarrow> hoare P (execute_instruction (load name type pointer align)) Q"
+  unfolding hoare_def by simp
+lemma [hoare_specs]: "hoare P (execute_add name wrap v1 v2) Q \<Longrightarrow> hoare P (execute_instruction (add name wrap type v1 v2)) Q"
+  unfolding hoare_def by simp
+lemma [hoare_specs]: "hoare P (execute_icmp name same_sign cond v1 v2) Q \<Longrightarrow> hoare P (execute_instruction (icmp name same_sign cond type v1 v2)) Q"
+  unfolding hoare_def by simp
+
+
+
+
+section "Block specifications"
+
+lemma block_phi_spec':
+  assumes "hoare ((\<lambda>s'. \<exists>p' v v'. p = Some p' \<and> map_of values p' = Some v \<and> register_\<alpha> s v = Some v' \<and> register_\<alpha> s' = (register_\<alpha> s)(reg name := Some v') \<and> memory_\<alpha> s' = memory_\<alpha> s)) (execute_block p (ps, is, t)) Q"
+  shows "hoare (\<lambda>s'. \<exists>p' v v'. s' = s \<and> distinct (map fst values) \<and> p = Some p' \<and> map_of values p' = Some v \<and> register_\<alpha> s v = Some v') (execute_block p ((phi name type values)#ps, is, t)) Q"
+  apply (rule hoare_intro)
+  apply (rule block_phi_wp_intro)
+  apply (rule phi_wp_intro)
+  using assms
+  apply (auto simp: state_marker_def)
+  apply blast
+  unfolding hoare_def
+  by blast
+
+lemma block_phi_spec[hoare_specs]:
+  assumes "hoare P (execute_phi p name values) x"
+  assumes "hoare x (execute_block p (ps, is, t)) Q"
+  shows "hoare P (execute_block p ((phi name type values)#ps, is, t)) Q"
+  apply (rule hoare_intro)
+  apply (rule wp_intro)
+  using assms
+  apply (auto simp: state_marker_def hoare_def consequence)
+  by (smt (verit, best) assms(2) consequence hoare_def)
+
+lemma block_instr_spec[hoare_specs]:
+  assumes "hoare P (execute_instruction i) x"
+  assumes "hoare x (execute_block p ([], is, t)) Q"
+  shows "hoare P (execute_block p ([], i#is, t)) Q"
+  apply (rule hoare_intro)
+  apply (intro wp_intro)
+  using assms
+  apply (auto simp: state_marker_def hoare_def consequence)
+  by (smt (verit, best) assms(2) consequence hoare_def)
+
+lemma block_ret_spec[hoare_specs]:
+  "hoare
+    (\<lambda>s'. \<exists>v. s' = s \<and> register_\<alpha> s value = Some v)
+    (execute_block p ([], [], ret type value))
+    (\<lambda>(s', r). \<exists>v. s' = s \<and> register_\<alpha> s value = Some v \<and> r = return_value v)"
+  apply (rule hoare_intro)
+  apply (rule block_ret_wp_intro)
+  by (auto simp: state_marker_def)
+
+lemma block_br_label_spec[hoare_specs]:
+  "hoare
+    (\<lambda>s'. s' = s)
+    (execute_block p ([], [], br_label l))
+    (\<lambda>(s', r). s' = s \<and> r = branch_label l)"
+  apply (rule hoare_intro)
+  apply (rule block_br_label_wp_intro)
+  by (auto simp: state_marker_def)
+
+lemma block_br_i1_spec[hoare_specs]:
+  "hoare
+    (\<lambda>s'. \<exists>b. s' = s \<and> register_\<alpha> s value = Some (vi1 b))
+    (execute_block p ([], [], br_i1 value l1 l2))
+    (\<lambda>(s', r). s' = s \<and> (\<exists>b. register_\<alpha> s value = Some (vi1 b) \<and> r = branch_label (if b then l1 else l2)))"
+  apply (rule hoare_intro)
+  apply (rule block_br_i1_wp_intro)
+  by (auto simp: state_marker_def)
+
+end
