Registers.thy
@@ -4,14 +4,14 @@ begin
 
 section "Simps"
 
-lemma memory_\<alpha>_eq[simp]: "memory_\<alpha> (vs,s,h) = memory_\<alpha> (vs',s,h)"
+lemma memory_\<alpha>_eq[simp]: "memory_\<alpha> (r,s,h) = memory_\<alpha> (r',s,h)"
   apply (rule ext)
   subgoal for x
     by (cases x; simp)
   done
 
 lemma register_\<alpha>_update_eq[simp]:
-  "register_\<alpha> (Mapping.update n v vs, s, h) = (register_\<alpha> (vs, s, h))(reg n := Some v)"
+  "register_\<alpha> (Mapping.update n v r, s, h) = (register_\<alpha> (r, s, h))(reg n := Some v)"
   apply (auto simp: fun_eq_iff split: llvm_value_ref.split)
   subgoal for x by (cases x; simp)
   done
@@ -21,17 +21,28 @@ lemma register_\<alpha>_val_eq[simp]:
   by (cases s; simp)
 
 
-section "Lemmas"
+
+section "register_\<alpha> operation"
+
+lemma set_register_\<alpha>:
+  "register_\<alpha> (set_register n v s) = (register_\<alpha> s)(reg n := Some v)"
+  apply (cases s; rule ext)
+  subgoal for r' s' h' x by (cases x; auto simp: set_register_value_def)
+  done
+
+
+
+section "Intro rules"
 
 named_theorems register_intro
 
 lemma wp_set_register_value_intro[THEN consequence, register_intro]:
-  "wp (return (set_register_value vs n v,s,h)) (\<lambda>s'. register_\<alpha> s' = (register_\<alpha> (vs,s,h))(reg n := Some v) \<and> memory_\<alpha> s' = memory_\<alpha> (vs,s,h))"
+  "wp (return (set_register_value n v r,s,h)) (\<lambda>s'. register_\<alpha> s' = (register_\<alpha> (r,s,h))(reg n := Some v) \<and> memory_\<alpha> s' = memory_\<alpha> (vs,s,h))"
   unfolding set_register_value_def
   by (intro wp_intro wp_return_intro; simp)
 
 lemma wp_set_register_intro[THEN consequence, wp_intro]:
-  shows "wp (return (set_register s n v)) (\<lambda>s'. register_\<alpha> s' = (register_\<alpha> s)(reg n := Some v) \<and> memory_\<alpha> s' = memory_\<alpha> s)"
+  shows "wp (return (set_register n v s)) (\<lambda>s'. register_\<alpha> s' = (register_\<alpha> s)(reg n := Some v) \<and> memory_\<alpha> s' = memory_\<alpha> s)"
   by (cases s; simp; intro wp_intro register_intro; simp)
 
 
